preparing next step, lemmas and necessary stuff. still unfinished

examples/AKE/AKE_proof2.ec
@@ -943,3 +943,623 @@ save.
 (* need symmetry rule for pRHL *)
 
 
+(*end proof: adding the collision check }*)
+
+(*{ enforcing freshness *)
+(* first, we introduce an operator that implements
+ the predicate fresh *)
+
+op fresh_op : Sid -> Event list-> bool.
+
+axiom fresh_op_def : forall s evs,
+fresh s evs <=> fresh_op s evs = true.
+
+
+
+local module AKE_Enforcement(FA : Adv2) = {
+  
+  var evs  : Event list               (* events for queries performed by adversary *)
+  var test : Sid option               (* session id of test session *)
+
+  var cSession, cH1, cH2 : int        (* counters for queries *)
+
+  var mH2 : (Sstring, Key) map        (* map for h2 *)
+  var sH2 : Sstring set               (* adversary queries for h2 *)
+
+  var mSk        : (Agent, Sk) map    (* map for static secret keys *)
+  var mEexp      : (Sidx, Eexp) map   (* map for ephemeral exponents of sessions *)
+  var mStarted   : (Sidx, Sdata2) map (* map of started sessions *)
+  var mCompleted : (Sidx, Epk)   map  (* additional data for completed sessions *)
+    
+  fun init() : unit = {
+    evs = [];
+    test = None;
+    cSession = 0;
+    cH1 = 0;
+    cH2 = 0;
+    mH2 = Map.empty;
+    sH2 = FSet.empty;
+    mSk = Map.empty;    
+    mEexp = Map.empty;
+    mStarted = Map.empty;
+    mCompleted = Map.empty;
+  }
+
+  module O : AKE_Oracles2 = {
+    
+    fun eexpRev(i : Sidx, a : Sk) : Eexp option = {
+      var r : Eexp option = None;
+      if (in_dom i mStarted && 
+    (let evs' = EphemeralRev(compute_psid mStarted mEexp i)::evs
+     in test <> None => fresh_op (proj test) evs' )) {
+        evs = EphemeralRev(compute_psid mStarted mEexp i)::evs;
+        if (sd2_actor(proj mStarted.[i]) = gen_pk(a)) {
+          r = mEexp.[i];
+        }
+      }
+      return r;
+    }
+    
+    fun h2(sstring : Sstring) : Key = {
+      var ke : Key;
+      ke = $sample_Key;
+      if (!in_dom sstring mH2) {
+        mH2.[sstring] = ke;
+      }
+      return proj mH2.[sstring];
+    }
+ 
+    fun h2_a(sstring : Sstring) : Key option = {
+      var r : Key option = None;
+      var ks : Key;
+      if (cH2 < qH2) {
+        cH2 = cH2 + 1;
+        sH2 = add sstring sH2;
+        ks = h2(sstring);
+        r = Some(ks);
+      }
+      return r;
+    }
+
+    fun init1(i : Sidx, A : Agent, B : Agent) : Epk option = {
+      var pX : Epk;
+      var r : Epk option = None; 
+      if (0 <= i < qSession && in_dom A mSk && 
+         in_dom B mSk && !in_dom i mStarted &&
+         ! collision_eexp_rcvd_op(Start((A,B,gen_epk(proj mEexp.[i]),init))::evs)) {
+        cSession = cSession + 1;
+        pX = gen_epk(proj mEexp.[i]);
+        mStarted.[i] = (A,B,init);
+        evs = Start((A,B,pX,init))::evs;
+        r = Some(pX);
+      }
+      return r;
+    }
+
+    fun resp(i : Sidx, B : Agent, A : Agent, X : Epk) : Epk option = {
+      var pY : Epk;
+      var r : Epk option = None;
+      if (0 <= i < qSession && in_dom A mSk && in_dom B mSk
+          && !in_dom i mStarted && !in_dom i mCompleted &&
+         ! collision_eexp_rcvd_op(Accept((B,A,gen_epk(proj mEexp.[i]),X,resp))::evs)) {
+        cSession = cSession + 1;
+        pY = gen_epk(proj mEexp.[i]);
+        mStarted.[i] = (B,A,resp);
+        mCompleted.[i] = X;
+        evs = Accept((B,A,pY,X,resp))::evs;
+        r = Some(pY);
+      }
+      return r;
+    }
+
+    fun init2(i : Sidx, Y : Epk) : unit = {
+      if (!in_dom i mCompleted && in_dom i mStarted &&
+      ! collision_eexp_rcvd_op(Accept(compute_sid mStarted mEexp mCompleted.[i <- Y] i)::evs)) {
+        mCompleted.[i] = Y;
+        evs = Accept(compute_sid mStarted mEexp mCompleted i)::evs;
+      }
+    }
+
+    fun staticRev(A : Agent) : Sk option = {
+      var r : Sk option = None;
+      if (in_dom A mSk &&
+      (let evs' = StaticRev A::evs
+       in test <> None => fresh_op (proj test) evs' )) {
+        r = mSk.[A];
+        evs = StaticRev(A)::evs;
+      }
+      return r;
+    }
+
+    fun computeKey(i : Sidx) : Key option = {
+      var r : Key option = None;
+      var a : Agent;
+      var b : Agent;
+      var ro : Role;
+      var k : Key;
+      if (in_dom i mCompleted) {
+        (a,b,ro) = proj mStarted.[i];
+        k = h2(gen_sstring (proj mEexp.[i]) (proj mSk.[a]) b (proj mCompleted.[i]) ro);
+        r = Some k;
+      }
+      return r;
+    }
+
+    fun sessionRev(i : Sidx) : Key option = {
+      var r : Key option = None;
+      if (in_dom i mCompleted &&
+     (let evs' = SessionRev
+          (compute_sid mStarted mEexp mCompleted i)::evs
+     in test <> None => fresh_op (proj test) evs' )) {
+        evs = SessionRev(compute_sid mStarted mEexp mCompleted i)::evs;
+        r = computeKey(i);
+      }
+      return r;
+    }
+  }
+  
+  module A = FA(O)
+
+  fun main() : bool = {
+    var b : bool = def;
+    var pks : Pk list = [];
+    var t_idx : Sidx = def;
+    var key : Key = def;
+    var keyo : Key option = def;
+    var b' : bool = def;
+    var i : int = 0;
+    var ska : Sk = def;
+    var pka : Pk = def;
+    var xa' : Eexp = def;
+    
+    init();
+    while (i < qAgent) {
+      ska = $sample_Sk;
+      pka = gen_pk(ska);
+      pks = pka :: pks;
+      mSk.[pka] = ska;
+    }
+    i = 0;
+    while (i < qSession) {
+      xa' = $sample_Eexp;
+      mEexp.[i] = xa';
+    } 
+
+    if (!collision_eexp_eexp_op mEexp) {
+     t_idx = A.choose(pks);
+     b = ${0,1};
+      if (mStarted.[t_idx] <> None && mCompleted.[t_idx] <> None) {
+      test = Some (compute_sid mStarted mEexp mCompleted t_idx);
+      (* the if-condition implies "mem (Accept (proj O.test)) O.evs" *)
+      if (b) {
+       keyo = O.computeKey(t_idx);
+      } else {
+       key  = $sample_Key;
+       keyo = Some key;
+      }
+      b' = A.guess(keyo);
+     }
+    }
+    return (b = b');
+  }
+}.
+
+(*{ Proof: enforcement doesn not make a difference
+    when we have fresh in the event *)
+
+
+
+lemma no_start_coll_mon : 
+forall e evs, 
+ (forall s, e <> Start s) =>
+ no_start_coll evs =>
+ no_start_coll (e :: evs).
+proof.
+ rewrite /no_start_coll; progress.
+ cut _ :  0 <> i.
+ apply not_def => heq.
+ generalize heq H3 => <-; rewrite nth_cons0 => h.
+ cut z:= H (A1, B1, X, r1).
+ by generalize z; rewrite -(proj_some (Start (A1, B1, X, r1))) -h proj_some.
+ cut _ : 0 <> j.
+ apply not_def => heq.
+ generalize heq H4 => <-; rewrite nth_cons0 => h.
+ cut z:= H (A2, B2, X, r2).
+ by generalize z; rewrite -(proj_some (Start (A2, B2, X, r2))) -h proj_some.
+ cut _: i - 1 = j - 1;last by smt.
+ apply (H0 X A1 A2 B1 B2 r1 r2 _ _ _ _ ); first 2 by smt.
+ by rewrite -H3 nth_consN  //.
+ by rewrite -H4 nth_consN  //.
+save.
+
+
+lemma no_accept_coll_mon : 
+forall e evs, 
+ (forall s, e <> Accept s) =>
+ no_accept_coll evs =>
+ no_accept_coll (e :: evs).
+proof.
+ rewrite /no_accept_coll; progress.
+ cut _ :  0 <> i.
+ apply not_def => heq.
+ generalize heq H5 => <-; rewrite nth_cons0 => h.
+ cut z:= H (A1, B1, X, Y1, r1).
+ by generalize z; rewrite -(proj_some (Accept (A1, B1, X, Y1, r1))) -h proj_some.
+ cut _ : 0 <> j.
+ apply not_def => heq.
+ generalize heq H6 => <-; rewrite nth_cons0 => h.
+ cut z:= H (A2, B2, X, Y2, r2).
+ by generalize z; rewrite -(proj_some (Accept (A2, B2, X, Y2, r2))) -h proj_some.
+ cut _: i - 1 = j - 1;last by smt.
+ apply (H0 X A1 A2 B1 B2 Y1 Y2 r1 r2 _ _ _ _ ).
+ by generalize H2; rewrite length_cons; smt.
+ by generalize H4; rewrite length_cons; smt.
+ by rewrite -H5 nth_consN  //.
+ by rewrite -H6 nth_consN  //.
+save.
+
+lemma n_exp_recvd_coll :
+ forall e evs,
+(forall ps, e <> Start ps) =>
+(forall s, e <> Accept s) =>
+! collision_eexp_rcvd evs => 
+! collision_eexp_rcvd (e :: evs). 
+proof.
+ intros => e evs hnstrt hnacc hcoll.
+ rewrite /collision_eexp_rcvd /=. 
+ apply not_def => [[i]] j s1 s2 s3 [hposi][hposj][hlength][hlt][hith] hor.
+ cut h: 0 <> i.
+  apply not_def => heq.
+  by generalize hith; rewrite -heq nth_cons0; smt.
+
+ cut h': 0 <> j.
+  apply not_def => heq.
+ generalize hor; rewrite -heq nth_cons0 => [[heq'] _ |[heq'] _ ].
+  cut abs := hnstrt s2.
+ by generalize abs;rewrite -(proj_some (Start s2)) -heq' proj_some.
+  by cut h' := hnacc s3; generalize h'; rewrite -(proj_some e) heq' proj_some.
+ cut: collision_eexp_rcvd evs; last by smt.
+ exists (i-1); exists (j-1); exists s1; exists s2; exists s3; progress; first 2 by smt.
+ by generalize hlength; rewrite length_cons; smt.
+ by smt.
+ by generalize hith; rewrite nth_consN; smt.
+ by generalize hor; rewrite nth_consN; smt. 
+save.
+
+pred start_evs_eexps evs (mEexps : (Sidx, Eexp) map) =
+forall s,  
+List.mem (Start s) evs => 
+exists e,
+in_dom e mEexps /\
+psid_sent s = gen_epk (proj (mEexps.[e])).
+
+lemma start_evs_eexps_emp : 
+forall m,
+start_evs_eexps [] m.
+proof.
+ intros => m; rewrite /start_evs_eexps; smt.
+save.
+
+lemma start_evs_eexps_pres :
+forall e evs m,
+start_evs_eexps evs m =>
+(forall s, e <> Start s) =>
+start_evs_eexps (e::evs) m.
+proof.
+ intros e evs m; rewrite /start_evs_eexps  => htl hneq s; rewrite mem_cons => [|] hor.
+ by cut _ := hneq s; smt.
+ by apply htl.
+save.
+
+lemma start_evs_eexps_pres_ev :
+forall evs m s,
+start_evs_eexps evs m =>
+(exists e, in_dom e m /\ psid_sent s = gen_epk (proj (m.[e]))) =>
+start_evs_eexps (Start s::evs) m.
+proof.
+ intros => evs m s; rewrite /start_evs_eexps => htl hex s'; 
+  rewrite mem_cons => [|] hor.
+ by cut ->: s' = s by apply Start_inj => //.
+ by apply htl. 
+save.
+
+
+pred accept_evs_eexps evs (mEexps : (Sidx, Eexp) map) =
+forall s,  
+List.mem (Accept s) evs => 
+exists e,
+in_dom e mEexps /\
+sid_sent s = gen_epk (proj (mEexps.[e])).
+
+lemma accept_evs_eexps_emp : 
+forall m,
+accept_evs_eexps [] m.
+proof.
+ intros => m; rewrite /accept_evs_eexps; smt.
+save.
+
+
+lemma accept_evs_eexps_pres :
+forall e evs m,
+accept_evs_eexps evs m =>
+(forall s, e <> Accept s) =>
+accept_evs_eexps (e::evs) m.
+proof.
+ intros e evs m; rewrite /accept_evs_eexps  => htl hneq s; rewrite mem_cons => [|] hor.
+ by cut _ := hneq s; smt.
+ by apply htl.
+save.
+
+lemma accept_evs_eexps_pres_ev :
+forall evs m s,
+accept_evs_eexps evs m =>
+(exists e, in_dom e m /\ sid_sent s = gen_epk (proj (m.[e]))) =>
+accept_evs_eexps (Accept s::evs) m.
+proof.
+ intros => evs m s; rewrite /accept_evs_eexps => htl hex s'; 
+  rewrite mem_cons => [|] hor.
+ by cut ->: s' = s by apply Accept_inj => //.
+ by apply htl. 
+save.
+
+
+lemma valid_accept_pres : 
+forall e evs, 
+valid_accepts evs =>
+(forall s, e <> Accept s) => 
+valid_accepts (e::evs).
+proof.
+ intros => e evs; rewrite /valid_accepts => htl hnotacc s i hith hrole.
+ case (0 = i) => hZ.
+   generalize hZ hith => <-; rewrite nth_cons0 => heq.
+   by cut h:= hnotacc s; generalize h; rewrite -(proj_some (Accept s)) -heq proj_some. 
+   
+   elim (htl s (i-1) _ _) => //;first by rewrite -hith nth_consN //.
+   intros => j [hlt][hll] hjth.
+   exists (j + 1); do split => //.
+   smt.
+   rewrite length_cons; smt.
+   rewrite -hjth nth_consN.
+
+cut _: !(i < 0).
+apply not_def => hi; generalize hith; rewrite nth_neg //; smt.
+smt.
+smt.
+save. 
+
+lemma valid_accept_pres_ev : 
+forall evs s, 
+valid_accepts evs =>
+mem (Start (psid_of_sid s)) evs =>
+valid_accepts (Accept s::evs).
+proof.
+  intros => evs s; rewrite /valid_accepts => htl hmem s' i hith hrole.
+  case (0 = i) => hZ.
+
+   generalize hZ hith => <-; rewrite nth_cons0 => heq.
+   cut heq': s = s'.  
+    by apply Accept_inj;rewrite -(proj_some (Accept s)) heq proj_some.
+   elim (mem_nth (Start (psid_of_sid s)) evs _) => // j [hbounds] hjth.
+   exists (j+1); do !split => //.
+    by smt.
+    by rewrite length_cons; smt.
+    by rewrite -heq' -hjth nth_consN; smt.
+
+   elim (htl s' (i-1) _ _) => //;first by rewrite -hith nth_consN //.
+   intros => j [hlt][hll] hjth.
+   exists (j + 1); do split => //.
+     by smt.
+     by rewrite length_cons; smt.
+
+     rewrite -hjth nth_consN.
+     cut _: !(i < 0).
+     apply not_def => hi; generalize hith; rewrite nth_neg //; smt.
+     smt. 
+     smt.
+save.
+
+pred inv_started evs (mStarted : (Sidx, Sdata2) map)
+                     (mEexp : (Sidx, Eexp) map)  =
+forall ps, 
+List.mem (Start ps) evs =>
+exists i,
+in_dom i mStarted /\
+in_dom i mEexp /\
+let (A, B, r) = proj (mStarted.[i]) in
+ps = (A, B, gen_epk (proj mEexp.[i]), r).
+
+lemma inv_started_pres :
+forall evs e m1 m2,
+inv_started evs m1 m2 =>
+(forall s, e <> Start s) =>
+inv_started (e::evs) m1 m2.
+proof.
+ intros => evs e m1 m2; rewrite /inv_started => htl hnstrt ps; 
+  rewrite mem_cons => [heq | hmem].
+  by cut:= hnstrt ps; smt. 
+  by apply (htl ps _); smt.
+save.
+ 
+(* pred inv_accepted evs (mCompleted : (Sidx, Sdata) map) *)
+(*                      (mEexp : (Sidx, Eexp) map)  = *)
+(* forall ps,  *)
+(* List.mem (Accept ps) evs => *)
+(* exists i, *)
+(* in_dom i mCompleted /\ *)
+(* in_dom i mEexp /\ *)
+(* let (A, B, X, Y, r) = proj (mCompleted.[i]) in *)
+(* ps = (A, B, X, Y, r). *)
+
+
+
+local equiv Eq_AKE_EexpRev_AKE_Enforcement :
+ AKE_Enforcement(A).main ~ AKE_NoColl(A).main  :
+true ==> 
+(res /\ test_fresh AKE_Enforcement.test AKE_Enforcement.evs
+                    /\ ! collision_eexp_eexp(AKE_Enforcement.mEexp) 
+                    /\ ! collision_eexp_rcvd(AKE_Enforcement.evs) ){1} <=>
+(res /\ test_fresh AKE_NoColl.test AKE_NoColl.evs
+                    /\ ! collision_eexp_eexp(AKE_NoColl.mEexp) 
+                    /\ ! collision_eexp_rcvd(AKE_NoColl.evs)){2}.
+proof.
+ fun.
+ seq 14 14:(={b,pks,t_idx,key,keyo,b',i,pks} /\
+  AKE_NoColl.evs{2} = AKE_Enforcement.evs{1} /\
+  AKE_NoColl.test{2} = AKE_Enforcement.test{1} /\
+  AKE_NoColl.cSession{2} = AKE_Enforcement.cSession{1} /\
+  AKE_NoColl.cH2{2} = AKE_Enforcement.cH2{1} /\
+  AKE_NoColl.mH2{2} = AKE_Enforcement.mH2{1} /\
+  AKE_NoColl.sH2{2} = AKE_Enforcement.sH2{1} /\
+  AKE_NoColl.mSk{2} = AKE_Enforcement.mSk{1} /\
+  AKE_NoColl.mEexp{2} = AKE_Enforcement.mEexp{1} /\
+  AKE_NoColl.mStarted{2} = AKE_Enforcement.mStarted{1} /\
+  AKE_NoColl.mCompleted{2} = AKE_Enforcement.mCompleted{1} /\
+  AKE_NoColl.evs{2} = []).
+ inline AKE_Enforcement(A).init AKE_NoColl(A).init.
+ eqobs_in  (true)
+  (AKE_NoColl.evs{2} = []) :
+  (={b,pks,t_idx,key,keyo,b',i,pks} /\
+  AKE_NoColl.evs{2} = AKE_Enforcement.evs{1} /\
+  AKE_NoColl.test{2} = AKE_Enforcement.test{1} /\
+  AKE_NoColl.cSession{2} = AKE_Enforcement.cSession{1} /\
+  AKE_NoColl.cH2{2} = AKE_Enforcement.cH2{1} /\
+  AKE_NoColl.mH2{2} = AKE_Enforcement.mH2{1} /\
+  AKE_NoColl.sH2{2} = AKE_Enforcement.sH2{1} /\
+  AKE_NoColl.mSk{2} = AKE_Enforcement.mSk{1} /\
+  AKE_NoColl.mEexp{2} = AKE_Enforcement.mEexp{1} /\
+  AKE_NoColl.mStarted{2} = AKE_Enforcement.mStarted{1} /\
+  AKE_NoColl.mCompleted{2} = AKE_Enforcement.mCompleted{1}).
+  by wp.
+  if=> //.
+   seq 2 2:(
+ ={b,pks,t_idx,key,keyo,b',i,pks} /\
+  AKE_NoColl.evs{2} = AKE_Enforcement.evs{1} /\
+  AKE_NoColl.test{2} = AKE_Enforcement.test{1} /\
+  AKE_NoColl.cSession{2} = AKE_Enforcement.cSession{1} /\
+  AKE_NoColl.cH2{2} = AKE_Enforcement.cH2{1} /\
+  AKE_NoColl.mH2{2} = AKE_Enforcement.mH2{1} /\
+  AKE_NoColl.sH2{2} = AKE_Enforcement.sH2{1} /\
+  AKE_NoColl.mSk{2} = AKE_Enforcement.mSk{1} /\
+  AKE_NoColl.mEexp{2} = AKE_Enforcement.mEexp{1} /\
+  AKE_NoColl.mStarted{2} = AKE_Enforcement.mStarted{1} /\
+  AKE_NoColl.mCompleted{2} = AKE_Enforcement.mCompleted{1} /\
+  AKE_NoColl.evs{2} = [] /\
+  ! collision_eexp_eexp_op AKE_NoColl.mEexp{2}).
+rnd.
+call (_ :
+   AKE_NoColl.evs{2} = AKE_Enforcement.evs{1} /\
+  AKE_NoColl.test{2} = AKE_Enforcement.test{1} /\
+  AKE_NoColl.cSession{2} = AKE_Enforcement.cSession{1} /\
+  AKE_NoColl.cH2{2} = AKE_Enforcement.cH2{1} /\
+  AKE_NoColl.mH2{2} = AKE_Enforcement.mH2{1} /\
+  AKE_NoColl.sH2{2} = AKE_Enforcement.sH2{1} /\
+  AKE_NoColl.mSk{2} = AKE_Enforcement.mSk{1} /\
+  AKE_NoColl.mEexp{2} = AKE_Enforcement.mEexp{1} /\
+  AKE_NoColl.mStarted{2} = AKE_Enforcement.mStarted{1} /\
+  AKE_NoColl.mCompleted{2} = AKE_Enforcement.mCompleted{1} /\
+  AKE_Enforcement.test{1} = None /\
+  !collision_eexp_rcvd(AKE_NoColl.evs{2}) /\
+  accept_evs_eexps AKE_NoColl.evs{2} AKE_NoColl.mEexp{2} /\
+  start_evs_eexps AKE_NoColl.evs{2} AKE_NoColl.mEexp{2} /\
+  no_start_coll(AKE_NoColl.evs{2}) /\
+  no_accept_coll(AKE_NoColl.evs{2}) /\
+  valid_accepts (AKE_NoColl.evs{2}) /\
+  inv_started AKE_NoColl.evs{2} AKE_NoColl.mStarted{2} AKE_NoColl.mEexp{2}  /\
+! collision_eexp_eexp_op AKE_NoColl.mEexp{2}).
+   fun; wp; skip; progress; try smt.
+    by apply n_exp_recvd_coll => //; smt.
+    by apply accept_evs_eexps_pres => //; smt.
+    by apply start_evs_eexps_pres => //; smt.
+    by apply no_start_coll_mon => //; smt. 
+    by apply no_accept_coll_mon => //; smt. 
+    by apply valid_accept_pres => //; smt. 
+    by apply inv_started_pres => //; smt.  
+    by apply n_exp_recvd_coll => //; smt.
+    by apply start_evs_eexps_pres => //; smt.
+    by apply no_start_coll_mon => //; smt. 
+    by apply no_accept_coll_mon => //; smt. 
+    by apply valid_accept_pres => //; smt.
+    by apply inv_started_pres => //; smt.  
+
+   by fun; sp; if => //; 
+    inline AKE_Enforcement(A).O.h2  AKE_NoColl(A).O.h2;
+    wp; rnd; wp; skip; progress => //.
+
+   fun; sp; if => //; wp; skip; progress; try smt.    
+a    by apply accept_evs_eexps_pres => //; smt.
+apply start_evs_eexps_pres_ev => //.
+exists i{2}; progress.
+
+   fun; sp; if => //.
+
+call 
+(_ :
+  (!fresh (proj AKE_NoColl.test) AKE_NoColl.evs),
+  (AKE_NoColl.evs{2} = AKE_Enforcement.evs{1} /\
+  AKE_NoColl.test{2} = AKE_Enforcement.test{1} /\
+  AKE_NoColl.cSession{2} = AKE_Enforcement.cSession{1} /\
+  AKE_NoColl.cH2{2} = AKE_Enforcement.cH2{1} /\
+  AKE_NoColl.mH2{2} = AKE_Enforcement.mH2{1} /\
+  AKE_NoColl.sH2{2} = AKE_Enforcement.sH2{1} /\
+  AKE_NoColl.mSk{2} = AKE_Enforcement.mSk{1} /\
+  AKE_NoColl.mEexp{2} = AKE_Enforcement.mEexp{1} /\
+  AKE_NoColl.mStarted{2} = AKE_Enforcement.mStarted{1} /\
+  AKE_NoColl.mCompleted{2} = AKE_Enforcement.mCompleted{1} /\
+
+  AKE_Enforcement.test{1} <> None),
+  AKE_Enforcement.test{1} <> None) => //.
+
+  by apply A_Lossless.
+  (* relational spec for eexpRev *)
+  fun.
+  seq 1 1: 
+( ! ! fresh (proj AKE_EexpRev.test{2}) AKE_EexpRev.evs{2} /\
+  ={i, a, r} /\
+  AKE_EexpRev.evs{2} = AKE_Enforcement.evs{1} /\
+  AKE_EexpRev.test{2} = AKE_Enforcement.test{1} /\
+  AKE_EexpRev.cSession{2} = AKE_Enforcement.cSession{1} /\
+  AKE_EexpRev.cH2{2} = AKE_Enforcement.cH2{1} /\
+  AKE_EexpRev.mH2{2} = AKE_Enforcement.mH2{1} /\
+  AKE_EexpRev.sH2{2} = AKE_Enforcement.sH2{1} /\
+  AKE_EexpRev.mSk{2} = AKE_Enforcement.mSk{1} /\
+  AKE_EexpRev.mEexp{2} = AKE_Enforcement.mEexp{1} /\
+  AKE_EexpRev.mStarted{2} = AKE_Enforcement.mStarted{1} /\
+  AKE_EexpRev.mCompleted{2} = AKE_Enforcement.mCompleted{1} /\
+  ! AKE_Enforcement.test{1} = None);first by wp.
+  if{1}.
+  by rcondt{2} 1 => //; wp; skip; progress; smt.
+  if{2} => //.
+  conseq (_ : _ ==>  ! AKE_Enforcement.test{1} = None /\ 
+                     ! fresh (proj AKE_EexpRev.test{2}) AKE_EexpRev.evs{2});first smt.
+  by wp; skip; progress => //;smt.
+
+  (* valid test preservation for eeexpreveal *)
+  by intros &2 hunfresh; fun; wp; skip; progress.
+  (* not fresh preservation for eeexpreveal *)
+  intros &1; fun; wp; skip; progress try smt.
+  generalize H.
+  rewrite !fresh_eq_notfresh.
+  cut h := 
+   notfresh_fresh (proj AKE_EexpRev.test{hr}) AKE_EexpRev.evs{hr} (EphemeralRev
+     (compute_psid AKE_EexpRev.mStarted{hr} AKE_EexpRev.mEexp{hr} i{hr})); smt. 
+  (* relational spec for h2 *)
+  fun;sp; if => //;inline AKE_Enforcement(A).O.h2  AKE_EexpRev(A).O.h2; wp; rnd; wp.
+  by skip; progress => //; smt.
+  (* valid test preservation for h2 *)
+  intros &2 hunfresh; fun.
+  inline AKE_Enforcement(A).O.h2; sp; if => //;wp; rnd => //;
+      first (by apply TKey.Dword.lossless).
+  by wp; skip; progress.
+  (* not fresh preservation for h2 *)
+  intros &1; fun.
+  inline AKE_EexpRev(A).O.h2; sp; if => //;wp; rnd => //;
+      first (by apply TKey.Dword.lossless).
+  by wp; skip; progress => //.
+  (* relational spec for Init1 *)
+  by fun; wp; skip; smt.
+  (* valid test preservation for Init1 *)
+  intros => &2 hfresh; fun; wp; skip; smt.
+  
+
+
+(* end proof: }*) 
